SystemFD/Evaluator/Soundness.lean
@@ -16,11 +16,14 @@ case _ Γ n _ om et =>
   symm at instsp; symm at ip;
   apply Red.inst nfh _ ip instsp; unfold Term.apply_spine; simp_all;
   unfold Ctx.is_openm; rw[om]; unfold Frame.is_openm; simp_all;
-case _ Γ n lt et => simp at et; rw [lt] at et; simp at et; sorry -- apply Red.letterm;
+case _ Γ n _ _ lt et =>
+    simp at et; rw [lt] at et; simp at et; subst et;
+    have nf :=  @Term.var_neutral_form n; symm at nf; symm at lt;
+    apply Red.letterm nf lt;
 case _ et => simp at et
 case _ et => simp at et; subst et; apply Red.beta
 case _ et => simp at et; subst et; apply Red.betat
-case _ et => simp at et; subst et; sorry -- apply Red.letterm;
+case _ Γ _ _ _ et => simp at et; subst et; apply Red.letbeta
 
 case _ Γ f t _ n sp _ t' om et =>
   simp at et; split at et;
@@ -32,7 +35,8 @@ case _ Γ f t _ n sp _ t' om et =>
     symm at ip; symm at instsp
     symm at et; symm at fnf;
     generalize tlp' : List.map (·.apply_spine sp) insts = tl' at *; symm at tlp'
-    have fred := Red.inst fnf sorry ip instsp tlp';
+    have omp : Γ.is_openm n := by unfold Ctx.is_openm; rw[om]; unfold Frame.is_openm; simp
+    have fred := Red.inst fnf omp ip instsp tlp';
     apply Red.app_congr fred; simp_all
   case _ =>
     rw[Option.bind_eq_some] at et;
@@ -105,45 +109,34 @@ case _ Γ p s b c ih et =>
       rw[Option.bind_eq_some] at site;
       cases site; case _ w h =>
       cases h; case _ h =>
-      injection (And.right h) with ts; subst ts;
-      -- apply Red.ite_congr (@ih w (And.left h)); trivial
-      sorry
-    -- case _ =>
-    -- simp_all; split at site;
-    case _ => simp_all; sorry
-      -- rw[Option.bind_eq_some] at site;
-      -- cases site; case _ w h =>
-      --   injection (And.right h) with ts; subst ts;
-      --   apply Red.ite_congr (@ih w (And.left h)); trivial
-  --case _ sp' sne snf x_stable => sorry
-     -- split at site;
-     -- case _ heq =>
-     --   -- rw[Option.bind_eq_some] at site;
-     --   split at site;
-     --   case _ w h =>
-     --     injection site with site; subst ts; symm at snf; symm at pne; rw[<-heq] at snf; symm at h;
-     --     apply Red.ite_matched pne snf h;
-     --     sorry
-     --   case _ => sorry
-    -- case _ neq => sorry
-       -- injection site with site; rw [<-site]; --  split at site;
-       -- simp at x_stable; symm at snf; symm at pne;
-       -- apply Red.ite_missed pne snf x_stable (Or.inl neq);
-         -- split at site;
-         -- case _  _ _ _ _ _ weqs =>
-         --   subst weqs; simp_all; split at site;
-         --   case _ px =>
-         --     injection site with br; rw[<-br]; symm at pne; symm at sne; symm at px;
-         --     apply Red.ite_matched pne sne px; apply Term.id_is_ctor ctor
-         --   case _ npx =>
-         --     injection site with site; subst site; symm at sne; symm at pne;
-         --     have _ :=  option_neg npx;
-         --     apply Red.ite_missed pne sne; simp_all
-         -- case _ cond =>
-         --   symm at pne; symm at sne;
-         --   injection site with ss ; subst ss;
-         --   simp_all; apply Red.ite_missed pne sne; simp_all;
-         -- case _ => simp at site
+      injection (And.right h) with ts; subst ts; simp at h;
+      apply Red.ite_congr (ih h); simp;
+    case _ snf =>
+      simp_all;
+      have wisctor := site.1;
+      replace site := site.2;
+      split at site;
+      case _ => rw[Option.bind_eq_some] at site; cases site; case _ w h =>
+        simp at h;
+        have tl' := h.2;
+        subst tl';
+        apply Red.ite_congr (ih h.1); simp;
+      case _ s'_stable =>
+        simp_all; split at site;
+        case _ headeqs =>
+          split at site;
+          case _ pfix =>
+            injection site with site; subst headeqs;
+            symm at snf; symm at pne; subst site; symm at pfix;
+            apply Red.ite_matched pne snf pfix wisctor;
+          case _ pfix =>
+             injection site with site; subst site; symm at snf; symm at pne;
+             have x :=  option_neg pfix;
+             apply Red.ite_missed pne snf s'_stable (Or.inr x)
+        case _ h =>
+          injection site with site; subst site;
+          symm at snf; symm at pne;
+          apply Red.ite_missed pne snf s'_stable (Or.inl h)
 
 -- GUARD
 case _ Γ p s c ih et =>
@@ -156,7 +149,8 @@ case _ Γ p s c ih et =>
   case _ =>
     rw[Option.bind_eq_some] at smatch;
     cases smatch; case _ s' smatch' =>
-    have ih' := @ih s' (And.left smatch'); simp_all
+    cases smatch'; case _ smatch' =>
+    have ih' := ih (And.left smatch'); simp_all
     have h' := And.right smatch'; subst h'; apply Red.guard_congr ih'; rfl
   case _ s' sp' snf =>
     split at smatch;
@@ -165,19 +159,29 @@ case _ Γ p s c ih et =>
       symm at snf; symm at frame_term; simp_all
       cases smatch;
       case _ w ts' =>
-        have ih' := @ih w (And.left ts'); simp_all
-        have h' := And.right ts'; subst h'; apply Red.guard_congr ih'; rfl
+        cases ts';
+        case _ ts' =>
+          have ih' := ih (And.left ts'); simp_all
+          have h' := And.right ts'; subst h'; apply Red.guard_congr ih'; rfl
     case _ =>
       simp_all; split at smatch;
-      case _ =>  sorry
-        -- cases smatch;
-        -- case _ w ts' =>
-        -- have ih' := @ih w (And.left ts'); simp_all
-        -- have h' := And.right ts'; subst h'; apply Red.guard_congr ih'; rfl
+      case _ s'_stable s_n =>
+        subst s_n; have s_is_inst := smatch.1; replace smatch := smatch.2;
+        split at smatch;
+        case _ pfix =>
+             injection smatch with smatch; subst smatch;
+             symm at snf; symm at pne; symm at pfix;
+             apply Red.guard_matched pne snf pfix;
+        case _ pfix =>
+             injection smatch with smatch; subst smatch; symm at snf; symm at pne;
+             have x :=  option_neg pfix;
+             apply Red.guard_missed pne snf s'_stable (Or.inr x)
       case _ xx heq =>
-        injection smatch with smatch; rw[<-smatch]; symm at pne; symm at snf;
-        have reds : Red Γ (.guard p s c) [] := (Red.guard_missed pne snf xx (Or.inl heq));
-        apply reds
+           have tl' := smatch.2; injection tl' with tl'; subst tl';
+           replace smatch := smatch.1;
+           symm at pne; symm at snf;
+           have reds : Red Γ (.guard p s c) [] := (Red.guard_missed pne snf xx (Or.inl heq));
+           apply reds
 
 case _ Γ _ et => simp at et; rw[<-et]; apply Red.sym
 case _ ih et =>
